basis/fsioProofScript.sml
@@ -9,13 +9,23 @@ val _ = new_theory"fsioProof";
 
 val _ = translation_extends "fsioProg";
 val _ = monadsyntax.add_monadsyntax();
+
+val WORD_UNICITY_R = Q.store_thm("WORD_UNICITY_R[xlet_auto_match]",
+`!f fv fv'. WORD (f :word8) fv ==> (WORD f fv' <=> fv' = fv)`, fs[WORD_def]);
+
 val IOFS_iobuff_def = Define`
   IOFS_iobuff =
-    SEP_EXISTS v. W8ARRAY iobuff_loc v * cond (LENGTH v = 258)
-`;
+    SEP_EXISTS v. W8ARRAY iobuff_loc v * cond (LENGTH v = 258) `;
 
 val IOFS_def = Define `
   IOFS fs = IOx fs_ffi_part fs * &(wfFS fs)`
+
+val IOFS_precond = Q.store_thm("IOFS_precond",
+  `wfFS fs ⇒
+   IOFS fs
+    {FFI_part (encode fs) (mk_ffi_next fs_ffi_part) (MAP FST (SND(SND fs_ffi_part))) events}`,
+  rw[IOFS_def,cfHeapsBaseTheory.IOx_def,fs_ffi_part_def,cfHeapsBaseTheory.IO_def,one_def]
+  \\ rw[set_sepTheory.SEP_EXISTS_THM,set_sepTheory.cond_STAR,set_sepTheory.SEP_CLAUSES]);
 
 val iobuff_loc = EVAL``iobuff_loc`` |> curry save_thm "iobuff_loc"
 
@@ -88,14 +98,7 @@ val STRING_FILENAME_UNICITY_L =
     (FILENAME f' fv <=> f' = f /\ ¬MEM #"\^@" (explode f) /\ strlen f < 256)`, 
   filename_tac);
 
-val fsupdate_unchanged = Q.store_thm("fsupdate_unchanged",
- `get_file_content fs fd = SOME(content, pos) ==> validFD fd fs ==>
-    fsupdate fs fd 0 pos content = fs`,
-    fs[fsupdate_def,get_file_content_def,validFD_def,IO_fs_component_equality]>>
-    rw[] >> pairarg_tac >> fs[ALIST_FUPDKEY_unchanged] >> rw[]);
-
 val basis_st = get_ml_prog_state;
-(* TODO: move copy/str_to_w8array elsewhere? *)
 
 val copyi_spec = Q.store_thm(
   "copyi_spec",
@@ -145,30 +148,12 @@ val str_to_w8array_spec = Q.store_thm(
   rpt strip_tac >> xcf "IO.str_to_w8array" (basis_st()) >>
   xlet_auto >- xsimpl >> xapp >> simp[]);
 
-(* TODO: add xlet_auto_match tag *)
-val eq_word8_v_thm =
-  mlbasicsProgTheory.eq_v_thm
-  |> DISCH_ALL
-  |> C MATCH_MP (ml_translatorTheory.EqualityType_NUM_BOOL
-                 |> CONJUNCTS |> el 4)
-                 |> Q.INST_TYPE [`:α` |->`:8`];
-val eq_num_v_thm =
-  mlbasicsProgTheory.eq_v_thm
-  |> DISCH_ALL
-  |> C MATCH_MP (ml_translatorTheory.EqualityType_NUM_BOOL
-                 |> CONJUNCTS |> el 1)
-                 |> Q.INST_TYPE [`:α` |->`:8`];
-
-
-val WORD_UNICITY_R = Q.store_thm("WORD_UNICITY_R[xlet_auto_match]",
-`!f fv fv'. WORD (f :word8) fv ==> (WORD f fv' <=> fv' = fv)`, fs[WORD_def]);
-
 val openIn_spec = Q.store_thm(
   "openIn_spec",
   `∀s sv fs.
      FILENAME s sv ∧
      CARD (FDOM (alist_to_fmap fs.infds)) < 255 ⇒
-     app (p:'ffi ffi_proj) ^(fetch_v "IO.open_in" (basis_st()))
+     app (p:'ffi ffi_proj) ^(fetch_v "IO.openIn" (basis_st()))
        [sv]
        (IOFS fs * IOFS_iobuff)
        (POST
@@ -177,19 +162,16 @@ val openIn_spec = Q.store_thm(
                   inFS_fname fs s) *
                 IOFS (openFileFS s fs 0))
           (\e. &(BadFileName_exn e ∧ ~inFS_fname fs s) * IOFS fs))`,
-  xcf "IO.open_in" (basis_st()) >>
+  xcf "IO.openIn" (basis_st()) >>
   fs[FILENAME_def, strlen_def, IOFS_def, IOFS_iobuff_def] >> 
-  xpull >>
-  rename [`W8ARRAY _ fnm0`] >>
+  xpull >> rename [`W8ARRAY _ fnm0`] >>
   qmatch_goalsub_abbrev_tac`catfs fs` >>
-  fs[iobuff_loc_def] >>
-  xlet_auto
+  fs[iobuff_loc_def] >> xlet_auto
   >- (xsimpl >> Cases_on`s` \\ fs[]) >>
   qabbrev_tac `fnm = insert_atI (MAP (n2w o ORD) (explode s) ++ [0w]) 0 fnm0` >>
   qmatch_goalsub_abbrev_tac`catfs fs' * _` >>
   Cases_on `inFS_fname fs s`
-  >- (
-    xlet `POSTv u2.
+  >- (xlet `POSTv u2.
             &(UNIT_TYPE () u2 /\ nextFD fs < 255 /\
               validFD (nextFD fs) (openFileFS s fs 0)) *
             W8ARRAY iobuff_loc (LUPDATE 0w 0 (LUPDATE (n2w (nextFD fs)) 1 fnm)) *
@@ -212,31 +194,24 @@ val openIn_spec = Q.store_thm(
         csimp[nextFD_ltX, openFileFS_def, openFile_def, validFD_def]) >>
     xlet_auto
     >- (xsimpl >> csimp[HD_LUPDATE] >> simp[Abbr`fnm`, LENGTH_insert_atI, LENGTH_explode]) >>
-    fs[iobuff_loc_def] >>
-    xlet_auto
+    fs[iobuff_loc_def] >> xlet_auto
     >- (xsimpl >> rw[Abbr`fnm`,LENGTH_insert_atI,LENGTH_explode,iobuff_loc,HD_LUPDATE]) >>
-    xlet_auto >- (xsimpl) >>
-    xif
-    >-(
-       xapp >> simp[fsioProgTheory.iobuff_loc_def] >> xsimpl >>
+    xlet_auto >- (xsimpl) >> xif
+    >-(xapp >> simp[fsioProgTheory.iobuff_loc_def] >> xsimpl >>
     fs[EL_LUPDATE,Abbr`fnm`,LENGTH_insert_atI,LENGTH_explode,wfFS_openFile,Abbr`fs'`]) >>
-    xlet_auto
-    >- (xcon >> xsimpl)
+    xlet_auto >- (xcon >> xsimpl)
     >- (xraise >> xsimpl >>
         sg `0 < LENGTH (LUPDATE (n2w (nextFD fs)) 1 fnm)`
         >-(
 	  fs[] >> fs[markerTheory.Abbrev_def] >> fs[] >>
-	  `0 + LENGTH (MAP (n2w ∘ ORD) (explode s) ++ [0w]) <= LENGTH fnm0` by (fs[LENGTH_explode]) >>
-	  fs[LENGTH_insert_atI]
-        ) >>
-        IMP_RES_TAC HD_LUPDATE >> fs[]
-      )
-  ) >>
+	  `0 + LENGTH (MAP (n2w ∘ ORD) (explode s) ++ [0w]) <= LENGTH fnm0` 
+        by (fs[LENGTH_explode]) >>
+	  fs[LENGTH_insert_atI]) >>
+        IMP_RES_TAC HD_LUPDATE >> fs[])) >>
   xlet `POSTv u2.
             &UNIT_TYPE () u2 * catfs fs *
             W8ARRAY iobuff_loc (LUPDATE 255w 0 fnm)`
-  >- (
-      simp[Abbr`catfs`,Abbr`fs'`] >> xffi >> simp[iobuff_loc_def] >>
+  >- (simp[Abbr`catfs`,Abbr`fs'`] >> xffi >> simp[iobuff_loc_def] >>
       simp[fsFFITheory.fs_ffi_part_def,IOx_def] >>
       qmatch_goalsub_abbrev_tac`IO st f ns` >>
       CONV_TAC(RESORT_EXISTS_CONV List.rev) >>
@@ -247,117 +222,58 @@ val openIn_spec = Q.store_thm(
 	   dimword_8, MAP_MAP_o, o_DEF, char_BIJ, wfFS_openFile,
 	   implode_explode, LENGTH_explode] >>
       simp[not_inFS_fname_openFile]) >>      
-  xlet_auto >-(xsimpl) >>
-  fs[iobuff_loc] >>
-  xlet_auto
+  xlet_auto >-(xsimpl) >> fs[iobuff_loc] >> xlet_auto
   >- (xsimpl >> csimp[HD_LUPDATE] >> simp[Abbr`fnm`, LENGTH_insert_atI, LENGTH_explode]) >>
-  xlet_auto >-(xsimpl) >>
-  xif
-  >-(
-     xapp >> xsimpl >> irule FALSITY >>
+  xlet_auto >-(xsimpl) >> xif
+  >-(xapp >> xsimpl >> irule FALSITY >>
      sg `0 < LENGTH fnm`
-     >-(
-       fs[markerTheory.Abbrev_def] >>
-       `0 + LENGTH (MAP (n2w ∘ ORD) (explode s) ++ [0w]) <= LENGTH fnm0` by (fs[LENGTH_explode]) >>
-       fs[LENGTH_insert_atI]
-     ) >>
+     >-(fs[markerTheory.Abbrev_def] >>
+        `0 + LENGTH (MAP (n2w ∘ ORD) (explode s) ++ [0w]) <= LENGTH fnm0` 
+            by (fs[LENGTH_explode]) >>
+        fs[LENGTH_insert_atI]) >>
      fs[HD_LUPDATE])>>
-  xlet_auto >-(xcon >> xsimpl) >>
-  xraise >> xsimpl >>
-  simp[BadFileName_exn_def]);
+  xlet_auto >-(xcon >> xsimpl) >> xraise >> xsimpl >> simp[BadFileName_exn_def]);
 
-val (eventually_rules,eventually_ind,eventually_cases) = Hol_reln`
-  (!ll. P ll ==> eventually P ll) /\
-  (!h t. ¬P (h:::t) /\ eventually P t ==> eventually P (h:::t)) `;
-
-val eventually_thm = store_thm(
-  "eventually_thm",
-  ``(eventually P [||] = P [||]) /\
-    (eventually P (h:::t) = (P (h:::t) \/(¬ P (h:::t) /\ eventually P t)))``,
-  CONJ_TAC THEN
-  CONV_TAC (LAND_CONV (ONCE_REWRITE_CONV [eventually_cases])) THEN
-  SRW_TAC [][]);
-
-val _ = export_rewrites ["eventually_thm"]
-
-val (always_rules,always_ind,always_cases) = Hol_reln`
-  (!h t. (P (h ::: t) /\ always P t) ==> always P (h ::: t)) `;
-
-val always_thm = store_thm(
-  "always_thm",
-  ``!h t. always P (h ::: t) = (P (h ::: t) /\ always P t) /\
-    ¬ always P [||]``,
-  rw[Once always_cases] >> rw[Once always_cases]);
-val _ = export_rewrites ["always_thm"]
-
-val always_eventually = Q.store_thm("always_eventually", 
-  `!ll. always (eventually P) ll ==> 
-    ?k. (P (THE (LDROP k ll)) /\ always(eventually P) (THE(LDROP k ll)))`,
-    HO_MATCH_MP_TAC always_ind >> 
-    rw[always_thm,eventually_thm] >>
-    qexists_tac`SUC k` >> fs[LDROP]);
-
-val always_eventually_ind = Q.store_thm("always_eventually_ind",
-  `(!ll. (P ll \/ (¬ P ll /\ Q (THE(LTL ll)))) ==> Q ll) ==>
-   !ll. always(eventually P) ll ==> Q ll`,
-   strip_tac >> HO_MATCH_MP_TAC always_ind >> rw[] >> fs[] >>
-   cases_on`P (h:::t)` >> fs[]);
-
-val always_DROP = Q.store_thm("always_DROP",
-  `!ll. always P ll ==> always P (THE(LDROP k ll))`,
-  Induct_on`k` >> cases_on`ll` >> fs[always_thm,LDROP]);
-  
-(* the filesystem will always eventually allow to write something *)
-val liveFS_def = Define`
-    liveFS fs = 
-        always (eventually (\ll. ?k. LHD ll = SOME k /\ k <> 0)) fs.numchars`
-
-val always_NOT_LFINITE = Q.store_thm("always_NOT_LFINITE",
-    `!ll. always P ll ==> ¬ LFINITE ll`,
-    HO_MATCH_MP_TAC always_ind >> rw[]);
-
-val LDROP_1 = Q.store_thm("LDROP_1",
-  `LDROP (1: num) (h:::t) = SOME t`,
-  `LDROP (SUC 0) (h:::t) = SOME t` by fs[LDROP] >>
-  metis_tac[ONE]);
-
-val wfFS_LDROP = Q.store_thm("wfFS_LDROP",
- `wfFS fs ==> LDROP k fs.numchars = SOME numchars' ==>
-    wfFS (fs with numchars := numchars')`,
- rw[wfFS_def] >> metis_tac[NOT_LFINITE_DROP_LFINITE]);
-
-val Lnext_def = tDefine "Lnext" `
-  Lnext P ll = if eventually P ll then
-                        if P ll then 0
-                        else SUC(Lnext P (THE (LTL ll)))
-                     else ARB` 
- (qexists_tac`(\(P,ll') (P',ll). 
-    P = P' /\ eventually P ll /\ eventually P ll' /\
-    LTL ll = SOME ll' /\ ¬ P ll)` >>reverse(rw[WF_DEF,eventually_thm])
-  >-(cases_on`ll` >> fs[])
-  >-(cases_on`ll` >> fs[]) >>
-  cases_on`w` >> rename[`B(P, ll)`] >> rename[`B(P, ll)`] >>
-  reverse(cases_on`eventually P ll`)
-  >-(qexists_tac`(P,ll)` >> rw[] >> pairarg_tac >> fs[] >> res_tac >> rfs[]) >>
-  rpt(LAST_X_ASSUM MP_TAC) >> qid_spec_tac `ll` >> 
-  HO_MATCH_MP_TAC eventually_ind >> rw[]
-  >-(qexists_tac`(P,ll)` >> rw[] >> pairarg_tac >> fs[] >> res_tac >> rfs[]) >>
-  cases_on`B(P,ll)` >-(metis_tac[]) >>
-  qexists_tac`(P,h:::ll)` >> fs[] >> rw[] >> pairarg_tac >> fs[]);
+(* openOut, openAppend here *)
 
 val validFD_ALOOKUP = Q.store_thm("validFD_ALOOKUP",
   `validFD fd fs ==> ?v. ALOOKUP fs.infds fd = SOME v`,
   rw[validFD_def] >> cases_on`ALOOKUP fs.infds fd` >> fs[ALOOKUP_NONE]);
 
-val Lnext_pos_def = Define`
-  Lnext_pos (ll :num llist) = Lnext (λll. ∃k. LHD ll = SOME k ∧ k ≠ 0) ll`
-
-val fsupdate_LTL = Q.store_thm("fsupdate_LTL",
-  `fs.numchars = h:::t ==>
-   fsupdate fs fd (SUC k) p c =
-   fsupdate (fs with numchars := t) fd k p c`,
-   rw[] >> fs[fsupdate_def,LDROP]);
-
+val close_spec = Q.store_thm(
+  "close_spec",
+  `∀(fdw:word8) fdv fs.
+     WORD fdw fdv ⇒  
+     app (p:'ffi ffi_proj) ^(fetch_v "IO.close" (basis_st())) [fdv]
+       (IOFS fs * IOFS_iobuff)
+       (POST (\u. &(UNIT_TYPE () u /\ validFD (w2n fdw) fs) *
+                 IOFS (fs with infds updated_by A_DELKEY (w2n fdw)))
+             (\e. &(InvalidFD_exn e /\ ¬ validFD (w2n fdw) fs) * IOFS fs))`,
+  xcf "IO.close" (basis_st()) >> simp[IOFS_def, IOFS_iobuff_def] >> xpull >>
+  rename [`W8ARRAY _ buf`] >> cases_on`buf` >> fs[] >>
+  xlet_auto >- xsimpl >> fs[LUPDATE_def] >>
+  xlet`POSTv uv. &(UNIT_TYPE () uv) *
+        W8ARRAY iobuff_loc ((if validFD (w2n fdw) fs then 1w else 0w) ::t) *
+        IOFS (if validFD (w2n fdw) fs then (fs with infds updated_by A_DELKEY (w2n fdw)) 
+                                      else fs)`
+  >-(xffi >> simp[iobuff_loc_def,IOFS_def,fsFFITheory.fs_ffi_part_def,IOx_def] >>
+     qmatch_goalsub_abbrev_tac`IO st f ns` >> xsimpl >>
+     qmatch_goalsub_abbrev_tac`wfFS fs' ∧ _` >>
+     CONV_TAC(RESORT_EXISTS_CONV List.rev) >>
+     map_every qexists_tac[`ns`,`f`,`encode fs'`,`st`] >> xsimpl >>
+     unabbrev_all_tac >> CASE_TAC >> rw[] >>
+     fs[mk_ffi_next_def, ffi_close_def, decode_encode_FS,
+        getNullTermStr_insert_atI, ORD_BOUND, ORD_eq_0,
+        dimword_8, MAP_MAP_o, o_DEF, char_BIJ, wfFS_openFile,
+        implode_explode, LENGTH_explode,closeFD_def,LUPDATE_def] 
+      >-(imp_res_tac validFD_ALOOKUP >> cases_on`fs` >> fs[IO_fs_infds_fupd])
+      >-(fs[validFD_def] >> imp_res_tac ALOOKUP_NONE >> fs[])) >>
+  NTAC 3 (xlet_auto >- xsimpl) >>
+  CASE_TAC >> xif >> instantiate
+  >-(xcon >> fs[IOFS_def] >> xsimpl) >>
+  xlet_auto >-(xcon >> xsimpl) >>
+  xraise >> fs[InvalidFD_exn_def,IOFS_def] >> xsimpl);
+      
 val writei_spec = Q.store_thm("writei_spec",
  `liveFS fs ⇒ wfFS fs ⇒ validFD (w2n fd) fs ⇒ 0 < n ⇒
   w2n fd < 255 ⇒ LENGTH rest = 255 ⇒ i + n <= 255 ⇒
@@ -472,19 +388,6 @@ val writei_spec = Q.store_thm("writei_spec",
     (fs[Lnext_pos_def,Once Lnext_def,liveFS_def]) >>
   fs[ADD] >> xsimpl);
 
-val fsupdate_o = Q.store_thm("fsupdate_o",
- `validFD fd fs ==> liveFS fs ==>
-  fsupdate (fsupdate fs fd k1 pos1 c1) fd k2 pos2 c2 = 
-  fsupdate fs fd (k1+k2) pos2 c2`,
-  rw[fsupdate_def,validFD_def]
-  >-(fs[ALIST_FUPDKEY_ALOOKUP] >>
-     CASE_TAC >> fs[ALOOKUP_NONE,ALIST_FUPDKEY_o,ALIST_FUPDKEY_eq])
-  >-(fs[ALIST_FUPDKEY_o] >> HO_MATCH_MP_TAC ALIST_FUPDKEY_eq >>
-	 rw[] >> cases_on`v` >> fs[]) >>
-  fs[LDROP_ADD,liveFS_def] >>
-  imp_res_tac always_NOT_LFINITE >> imp_res_tac NOT_LFINITE_DROP >>
-  FIRST_X_ASSUM(ASSUME_TAC o Q.SPEC`k1`) >> fs[]);
-
 val insert_atI_insert_atI = Q.store_thm("insert_atI_insert_atI",
   `pos2 = pos1 + LENGTH c1 ==>
     insert_atI c2 pos2 (insert_atI c1 pos1 l) = insert_atI (c1 ++ c2) pos1 l`,
@@ -492,7 +395,6 @@ val insert_atI_insert_atI = Q.store_thm("insert_atI_insert_atI",
        GSYM DROP_DROP_T,DROP_LENGTH_TOO_LONG,DROP_LENGTH_NIL_rwt]
     >> fs[DROP_LENGTH_NIL_rwt,LENGTH_TAKE,DROP_APPEND1,TAKE_APPEND,TAKE_TAKE,
        DROP_DROP_T,DROP_APPEND2,TAKE_LENGTH_TOO_LONG,TAKE_SUM,LENGTH_DROP]);
-
 
 val write_spec = Q.store_thm("write_spec",
  `!n fs i pos h1 h2 h3 rest bc fdv nv iv fd content.
@@ -541,7 +443,6 @@ val write_spec = Q.store_thm("write_spec",
   PURE_REWRITE_TAC[Once (Q.SPECL [`i`,`nw`] ADD_COMM)] >>
   fs[Once ADD_COMM,GSYM DROP_DROP_T,take_drop_partition,MAP_DROP]);
 
-
 val write_char_spec = Q.store_thm("write_char_spec",
   `!(fd :word8) fdv c cv bc content pos.
     liveFS fs ⇒ wfFS fs ⇒
@@ -570,59 +471,13 @@ val write_char_spec = Q.store_thm("write_char_spec",
   xcon >> fs[IOFS_iobuff_def] >> xsimpl >> rw[] >>
   fs[CHR_ORD,LESS_MOD,ORD_BOUND] >> qexists_tac`k` >> xsimpl);
 
-val LENGTH_extract_aux = Q.store_thm("LENGTH_extract_aux",
-`!s x y. LENGTH (extract_aux s x y) = y`,
-     Induct_on`y` >> fs[extract_aux_def,MIN_DEF]);
-
-val strlen_extract_le = Q.store_thm("strlen_extract_le",
-`!s x y. strlen (extract s x y) <= strlen s - x`,
-  rw[extract_def] >> CASE_TAC >> fs[LENGTH_extract_aux]);
-
-val extract_aux_DROP = Q.store_thm("extract_aux_DROP",
-  `!s k. extract_aux (strlit s) k (LENGTH s - k) = DROP k s`,
-  rw[] >> `?n. STRLEN s - k = n` by fs[] >>
-  FIRST_X_ASSUM MP_TAC >> qid_spec_tac`s` >> qid_spec_tac`k` >>
-  induct_on`n` >> fs[extract_aux_def,STRLEN_DEF,DROP_EL_CONS] >>
-  rw[] >> fs[extract_aux_def,DROP_LENGTH_TOO_LONG] >>
-  (* simplify *)
-  FIRST_X_ASSUM MP_TAC >> PURE_REWRITE_TAC [Once (GSYM SUB_EQ_0)] >>
-  strip_tac >> FIRST_X_ASSUM (fn x => PURE_REWRITE_TAC[x]) >>
-  fs[extract_aux_def])
-
-val extract_aux_eq = Q.store_thm("extract_aux_eq",
-  `!n s. n = LENGTH s ==>
-   extract_aux (strlit s) 0 n = s`,
-  rw[] >> ASSUME_TAC(Q.SPECL[`s`,`0`] extract_aux_DROP) >> fs[]);
-
-val extract_aux_add_r = Q.store_thm("extract_aux_add_r",
-  `!n1 n2 s i. extract_aux s i (n1 + n2) = 
-                extract_aux s i n1 ++ extract_aux s (i+n1) n2`,
-  induct_on`n1` >- fs[extract_aux_def] >>
-  rw[] >> fs[GSYM ADD_SUC,extract_aux_def] >> fs[ADD1]);
-
-val extract_aux_eq = Q.store_thm("extract_aux_eq",
-  `!s n. n = LENGTH s ==>
-   extract_aux (strlit s) 0 n =s`,
-  rw[] >> ASSUME_TAC(Q.SPECL[`s`,`0`] extract_aux_DROP) >> fs[]);
-
-val extract_aux_TAKE = Q.store_thm("extract_aux_TAKE",
-  `!s. n <= LENGTH s ==>
-     extract_aux (strlit s) 0 n = TAKE n s`,
-  rw[] >>
-  sg`extract_aux (strlit s) 0 n ++ extract_aux (strlit s) n (LENGTH s - n)  = 
-     TAKE n s ++ DROP n s`
-  >-(fs[TAKE_DROP, GSYM extract_aux_add_r] >>
-     ASSUME_TAC(Q.SPECL[`n`,`STRLEN s - n`,`strlit s`,`0`]extract_aux_add_r) >>
-     rfs[] >> fs[extract_aux_eq]) >>
-  FIRST_X_ASSUM MP_TAC >> PURE_REWRITE_TAC[extract_aux_DROP] >> rw[]);
-
-val write_string_spec = Q.store_thm("write_string_spec",
+val output_spec = Q.store_thm("output_spec",
   `!s (fd :word8) fdv sv fs content pos. 
     WORD fd fdv ⇒ validFD (w2n fd) fs ⇒ 
     STRING_TYPE s sv ⇒
     liveFS fs ⇒ w2n fd < 255 ⇒  wfFS fs ⇒
     (get_file_content fs (w2n fd) = SOME(content, pos)) ⇒
-    app (p:'ffi ffi_proj) ^(fetch_v "IO.write_string" (basis_st())) [fdv; sv]
+    app (p:'ffi ffi_proj) ^(fetch_v "IO.output" (basis_st())) [fdv; sv]
     (IOFS fs * IOFS_iobuff)  
     (POSTv uv. &(UNIT_TYPE () uv) * IOFS_iobuff * 
        SEP_EXISTS k. IOFS (fsupdate fs (w2n fd) k (pos + (strlen s))
@@ -631,7 +486,7 @@ val write_string_spec = Q.store_thm("write_string_spec",
   `?n. strlen s <= n` by (qexists_tac`strlen s` >> fs[]) >>
   FIRST_X_ASSUM MP_TAC >> qid_spec_tac`s` >>
   Induct_on`n` >>
-  xcf "IO.write_string" (basis_st()) >> fs[IOFS_iobuff_def] >>
+  xcf "IO.output" (basis_st()) >> fs[IOFS_iobuff_def] >>
   xpull >> rename [`W8ARRAY _ buff`] >>
   Cases_on `buff` >> fs[] >> qmatch_goalsub_abbrev_tac`h1 :: t` >>
   Cases_on `t` >> fs[] >> qmatch_goalsub_abbrev_tac`h1 :: h2 :: rest'` >>
@@ -749,6 +604,135 @@ val read_char_spec = Q.store_thm("read_char_spec",
   xapp >> xsimpl >>
   `nr = 1` by fs[] >> fs[] >> xsimpl >> 
   fs[take1_drop,eof_def,get_file_content_def] >> pairarg_tac >> fs[]);
- 
+
+(* Standard IO *)
+
+(* standatd nput has file descriptor 0 *)
+val STDIN_def = Define`
+    STDIN input = IOFS_iobuff * SEP_EXISTS fs pos. IOFS fs * &liveFS fs *
+      &(get_file_content fs 0 = SOME(input, pos))` 
+
+(* standatd output has file descriptor 1 and the position is at the end *)
+val STDOUT_def = Define`
+    STDOUT output = IOFS_iobuff * SEP_EXISTS fs. IOFS fs * &liveFS fs *
+      &(get_file_content fs 1 = SOME(output,LENGTH output))` 
+
+(* standatd error has file descriptor 2 and the position is at the end *)
+val STDERR_def = Define`
+    STDERR output = IOFS_iobuff * SEP_EXISTS fs. IOFS fs * &liveFS fs *
+      &(get_file_content fs 2 = SOME(output,LENGTH output))` 
+
+val encode_fds_11 = Q.store_thm("encode_fds_11",
+  `encode_fds l1 = encode_fds l2 ⇒ l1 = l2`,
+  rw[] >> `decode_fds (encode_fds l1) = decode_fds(encode_fds l2)` by fs[] >>
+  fs[decode_encode_fds]);
+
+val encode_files_11 = Q.store_thm("encode_files_11",
+  `encode_files l1 = encode_files l2 ⇒ l1 = l2`,
+  rw[] >> 
+  `decode_files (encode_files l1) = decode_files(encode_files l2)` by fs[] >>
+  fs[decode_encode_files]);
+
+val UNIQUE_IOFS = Q.store_thm("UNIQUE_IOFS",
+`!s. VALID_HEAP s ==> !fs1 fs2 H1 H2. (IOFS fs1 * H1) s /\
+                                      (IOFS fs2 * H2) s ==> fs1 = fs2`,
+  rw[IOFS_def,IOFS_def,cfHeapsBaseTheory.IOx_def, fs_ffi_part_def,
+     GSYM STAR_ASSOC,encode_def] >>
+  IMP_RES_TAC FRAME_UNIQUE_IO >> 
+  fs[encode_files_11,encode_fds_11,IO_fs_component_equality]);
+
+val STDIN_FFI_part_hprop = Q.store_thm("STDIN_FFI_part_hprop",
+  `FFI_part_hprop (STDIN x)`,
+  rw [STDIN_def,IOFS_def,
+      cfHeapsBaseTheory.IO_def, cfHeapsBaseTheory.IOx_def,
+      fs_ffi_part_def, cfMainTheory.FFI_part_hprop_def,
+    set_sepTheory.SEP_CLAUSES,set_sepTheory.SEP_EXISTS_THM,
+    cfHeapsBaseTheory.W8ARRAY_def,IOFS_iobuff_def,
+    cfHeapsBaseTheory.cell_def]
+  \\ fs[set_sepTheory.one_STAR,STAR_def]
+  \\ imp_res_tac SPLIT_SUBSET >> fs[SUBSET_DEF]
+  \\ metis_tac[]);
+
+val STDOUT_FFI_part_hprop = Q.store_thm("STDOUT_FFI_part_hprop",
+  `FFI_part_hprop (STDOUT x)`,
+  rw [STDOUT_def,IOFS_def,
+      cfHeapsBaseTheory.IO_def, cfHeapsBaseTheory.IOx_def,
+      fs_ffi_part_def, cfMainTheory.FFI_part_hprop_def,
+    set_sepTheory.SEP_CLAUSES,set_sepTheory.SEP_EXISTS_THM,
+    cfHeapsBaseTheory.W8ARRAY_def,IOFS_iobuff_def,
+    cfHeapsBaseTheory.cell_def]
+  \\ fs[set_sepTheory.one_STAR,STAR_def]
+  \\ imp_res_tac SPLIT_SUBSET >> fs[SUBSET_DEF]
+  \\ metis_tac[]);
+  
+val STDERR_FFI_part_hprop = Q.store_thm("STDERR_FFI_part_hprop",
+  `FFI_part_hprop (STDERR x)`,
+  rw [STDERR_def,IOFS_def,
+      cfHeapsBaseTheory.IO_def, cfHeapsBaseTheory.IOx_def,
+      fs_ffi_part_def, cfMainTheory.FFI_part_hprop_def,
+    set_sepTheory.SEP_CLAUSES,set_sepTheory.SEP_EXISTS_THM,
+    cfHeapsBaseTheory.W8ARRAY_def,IOFS_iobuff_def,
+    cfHeapsBaseTheory.cell_def]
+  \\ fs[set_sepTheory.one_STAR,STAR_def]
+  \\ imp_res_tac SPLIT_SUBSET >> fs[SUBSET_DEF]
+  \\ metis_tac[]);
+open mllistProgTheory
+
+(* `(UNIT_TYPE --> WORD) (\u. 0w) (^(fetch_v "IO.stdin" (basis_st())))` *)
+
+val stdin_spec = Q.store_thm("stdin_spec",
+  `UNIT_TYPE () uv ⇒
+   app (p:'ffi ffi_proj) ^(fetch_v "IO.stdin" (basis_st())) [uv]
+   (emp) (POSTv v. &WORD (0w:word8) v)`,
+  xcf "IO.stdin" (basis_st()) >> xmatch >> fs[UNIT_TYPE_def] >>
+  rw[] >-(xapp >> xsimpl) >> EVAL_TAC);
+
+val stdout_spec = Q.store_thm("stdout_spec",
+  `UNIT_TYPE () uv ⇒
+   app (p:'ffi ffi_proj) ^(fetch_v "IO.stdout" (basis_st())) [uv]
+   (emp) (POSTv v. &WORD (1w:word8) v)`,
+  xcf "IO.stdout" (basis_st()) >> xmatch >> fs[UNIT_TYPE_def] >>
+  rw[] >-(xapp >> xsimpl) >> EVAL_TAC);
+
+val stderr_spec = Q.store_thm("stderr_spec",
+  `UNIT_TYPE () uv ⇒
+   app (p:'ffi ffi_proj) ^(fetch_v "IO.stderr" (basis_st())) [uv]
+   (emp) (POSTv v. &WORD (2w:word8) v)`,
+  xcf "IO.stderr" (basis_st()) >> xmatch >> fs[UNIT_TYPE_def] >>
+  rw[] >-(xapp >> xsimpl) >> EVAL_TAC);
+
+(* use earlier *)
+val get_file_content_validFD = Q.store_thm("get_file_content_validFD",
+  `get_file_content fs fd = SOME(c,p) ⇒ validFD fd fs`,
+  fs[get_file_content_def,validFD_def] >> rw[] >> pairarg_tac >>
+  imp_res_tac ALOOKUP_MEM >> fs[ALOOKUP_MEM,MEM_MAP] >> instantiate);
+
+val liveFS_fsupdate = Q.store_thm("liveFS_fsupdate",
+  `liveFS fs ⇒ liveFS (fsupdate fs fd k i c)`,
+  fs[liveFS_def,fsupdate_def,always_DROP]);
+
+val get_file_content_fsupdate = Q.store_thm("get_file_content_fsupdate",
+  `get_file_content fs fd = SOME u ⇒
+  get_file_content (fsupdate fs fd x i c) fd = SOME(c,i)`,
+  rw[get_file_content_def, fsupdate_def] >>
+  pairarg_tac >> fs[ALIST_FUPDKEY_ALOOKUP]);
+
+val insert_atI_end = Q.store_thm("insert_atI_end",
+  `insert_atI l1 (LENGTH l2) l2 = l2 ++ l1`,
+  simp[insert_atI_def,DROP_LENGTH_TOO_LONG]);
+
+val print_spec = Q.store_thm("print_spec",
+  `!s sv fs output. 
+    STRING_TYPE s sv ⇒
+    app (p:'ffi ffi_proj) ^(fetch_v "IO.print" (basis_st())) [sv]
+    (STDOUT output)  
+    (POSTv uv. &(UNIT_TYPE () uv) * STDOUT (STRCAT output (explode s)))`,
+  xcf "IO.print" (basis_st()) >> fs[STDOUT_def,IOFS_def] >> xpull >>
+  xlet_auto >-(xcon >> xsimpl) >> xlet_auto >- xsimpl >>
+  xapp >> fs[get_file_content_validFD,IOFS_def] >> xsimpl >> instantiate >>
+  fs[get_file_content_validFD,IOFS_def] >> xsimpl >> rw[] >> instantiate >>
+  fs[wfFS_fsupdate,liveFS_fsupdate,get_file_content_fsupdate,insert_atI_end,
+     LENGTH_explode] >> xsimpl);
+
 val _ = export_theory();
 
